\appendix

\section{Squeeze functions}
To bound~$1-\Psi(x \given b)$, let,
\begin{align}
1-\Psi(x \given b) 
  &=
    \sum_{n=0}^\infty (-1)^n \frac{\Gamma(n+b)}{\Gamma(n+1)} \frac{2n+b}{\Gamma(b+1)}
    \exp\left\{- \frac{2n(n+b)}{x} \right\} \\
  &= \sum_{n=0}^\infty (-1)^n \psi_n(x \given b).
\end{align}
We have,
\begin{align}
\frac{1}{n} \leq \frac{\Gamma(n+b)}{\Gamma(n+1)} \leq \frac{1}{n^{1-b}} \leq 1,
\end{align}
and,
\begin{align}
1 \leq \frac{1}{\Gamma(b+1)} \leq 1.13,
\end{align}
for~$b \in [0,1]$. Finally,
\begin{align}
1 - \frac{2n(n+b)}{x} \leq \exp \left\{ - \frac{2n(n+b)}{x}   \right\} \leq 1 - \frac{n(n+b)}{x}.
\end{align}
Together these imply,
\begin{align}
\frac{1}{n} \left( 1 - \frac{2n(n+b)}{x} \right) \leq 
&\psi_n(x \given b) \leq
\frac{1.13}{n^{1-b}} \left( 1 - \frac{n(n+b)}{x} \right)  \leq 
1.13 \left( 1 - \frac{n(n+b)}{x} \right) \\
\frac{1}{n} -\frac{2(n+b)}{x} \leq 
&\psi_n(x \given b) \leq
\frac{1.13xn^b - n^{b+1}(n+b)}{n x } \leq 
1.13 -\frac{1.13 n(n+b)}{x}
\end{align}
To get a lower bound on~${1-\Psi(x \given b)}$, we lower bound the even terms 
and upper bound the odd (negated) terms.
For the weaker upper bound, we have,
\begin{align}
1-\Psi(x \given b) 
  &= 1 + \sum_{j=0}^\infty \psi_{2j+2}(x \given b) - \psi_{2j+1}(x \given b) \\
  &\leq 1 + \sum_{j=0}^\infty 1.13 - \frac{(2j+2)(2j+2+b)}{x} - \frac{1}{2j+1} + \frac{2(2j+1+b)}{x} \\
  &= 1 + \sum_{j=0}^\infty \frac{1.13(2j+1)-1}{2j+1} + \frac{4j+2+2b - (2j+2)(2j+2+b)}{x} \\ 
  &= 1 + \sum_{j=0}^\infty \frac{1.13(2j+1)-1}{2j+1} + \frac{4j+2+2b - 2j^2 -4j -2jb -4j - 4 -2b}{x} \\
  &= 1 + \sum_{j=0}^\infty \frac{1.13(2j+1)-1}{2j+1} + \frac{-2j^2 -2j(2+b) - 2}{x}
\end{align}
% \begin{align}
% 1 - \Psi(x \given b) &= 1 + \sum_{n=1}^\infty (-1)^n \psi_n(x \given b) \\
%   &\leq 1 + \sum_{n=1}^\infty - \frac{1.13xn^b - n^{b+1}(n+b)}{n x} + \frac{x - 2(n+1)(n+1+b)}{(n+1)x} \\ 
% &= 1 + \sum_{n=1}^\infty \frac{-1.13xn^b(n+1) + n^{b+1}(n+1)(n+b) + xn - 2n(n+1)(n+1+b)}{n(n+1)x} \\
% &= 1 + \sum_{n=1}^\infty \frac{-1.13n^{b}}{(n+1)} + \frac{-1.13n^b}{n(n+1)} 
% + \frac{n^{b}(n+b)}{x} + \frac{1}{(n+1)} - \frac{2(n+1+b)}{x}
% \end{align}

\section{Series expansion of~$\Psi(x \given b)$}

\begin{align}
((-1)^n (b+2 n) \Gamma(b+n))/(\Gamma(b+1) \Gamma(n+1))
-(2 ((-1)^n n (b+n) (b+2 n) \Gamma(b+n)))/(x (\Gamma(b+1) \Gamma(n+1)))
+(2 (-1)^n n^2 (b+n)^2 (b+2 n) \Gamma(b+n))/(x^2 \Gamma(b+1) \Gamma(n+1))
-(4 ((-1)^n n^3 (b+n)^3 (b+2 n) \Gamma(b+n)))/(3 x^3 (\Gamma(b+1) \Gamma(n+1)))
+(2 (-1)^n n^4 (b+n)^4 (b+2 n) \Gamma(b+n))/(3 x^4 \Gamma(b+1) \Gamma(n+1))
+O((1/x)^5)
\end{align}

\section{Trying to approximate the density}

\begin{align}
\psi(x \given b) = \frac{\mathrm{d} \Psi(x \given b)}{\mathrm{d} x} &= 
    \sum_{n=0}^\infty (-1)^{n+1} \frac{\Gamma(n+b)}{\Gamma(n+1)} \frac{2n+b}{\Gamma(b+1)}
    \left( \frac{2n(n+b)}{x^2}\right) \exp\left\{- \frac{2n(n+b)}{x} \right\}  \\
  &= \frac{2}{b} x^{-2} \sum_{n=0}^\infty (-1)^{n+1} \frac{(2n+b)(n+b)}{\mathrm{B}(n,b)}
     \exp\left\{- \frac{2n(n+b)}{x} \right\}  
\end{align}

I think the sum (with the exception of the~$x^{-3/2}$ term) should look approximately like
~$e^{-cx}$ for~$x>1$. 
\begin{align}
  \distJacobi(x \given b) &= \frac{2^b}{\Gamma(b)} \frac{1}{\sqrt{2\pi x^3}}
  \sum_{n=0}^\infty (-1)^n \frac{\Gamma(n+b)}{\Gamma(n+1)} (2n+b)
  \exp\left\{- \frac{(2n+b)^2}{2x} \right\} 
\end{align}
For~$n \geq 1$, the ratio of gamma functions is bounded by,
\begin{align}
\frac{\Gamma(n+b)}{\Gamma(n+1)} &\geq \frac{\Gamma(n)}{\Gamma(n+1)} 
= \frac{\Gamma(n)}{n\Gamma(n)} = \frac{1}{n}.
\end{align}
The ratio of gamma functions looks something like, 
\begin{align}
\frac{\Gamma(n+b)}{\Gamma(n+1)} &= \exp\left\{ \log \Gamma(n+b) - \log \Gamma(n+1) \right\} \\
&\approx \exp \left\{ (n+b) \log (n+b) - (n+b) - [(n+1)\log(n+1) -(n+1)] \right\} \\
&\approx \exp \left\{ (n+b) (\log n + b/n) - (n+b) - [(n+1) (\log n + 1/n)  -(n+1)] \right\} \\
&= \exp \left\{ (n+b-n-1) \log n + (n+b)(b/n-1)  - (n+1)(1/n -1) \right\} \\
&= \exp \left\{ (b-1) \log n + b -n +b^2/n -b - (1 -n + 1/n -1  )   \right\} \\
&= \exp \left\{ (b-1) \log n - \frac{1-b^2}{n}   \right\} \\
&= \frac{1}{n^{1-b}} e^{-\frac{1-b^2}{n}}
\end{align}
Where we made the approximation,~$\log(n+b) \approx \log n + b/n$
When~$b=1$ these terms are obviously equal and their ratio is 1. 
When~$b=0$ the ratio is equal to~$n^{-1}$. For intermediate values,
the ratio has to be somewhere in between. 
We can make this more precise with Stirling's approximation.

\section{Laplace transforms}
\begin{align}
  &= 
\left( \frac{
\left(\exp \{z \}+1 \right) 
\left( 2 \exp \left\{ \sqrt{\frac{z^2/2 +t}{2}}\right\} \right)}  
{ \left( 2 \exp \left\{ \frac{z}{2} \right\}\right) 
\left(\exp \left\{ 2\sqrt{\frac{z^2/2 +t}{2}}\right\}+1 \right)}
\right)^b \\
  &= \left(   \frac{
2 \left[\exp \left\{ z+ \sqrt{\frac{z^2/2 +t}{2}}\right\} + \exp \{\sqrt{\frac{z^2/2 +t}{2}} \} \right]}
{ 
2 \left[\exp \left\{ z/2+ 2\sqrt{\frac{z^2/2 +t}{2}}\right\} + \exp \{z/2 \} \right]
}
\right)^b
\end{align}
